\section{均方误差}

\subsection{回归估计量的均方误差}
\begin{theorem}
	回归估计量的均方误差为：
	\begin{align*}
		MSE(\hat{\mu}_{Y_{reg}})&= 
		E\left\lbrace\big[\bar{y}+\hat{B}_1(\mu_X-\bar{x})-\mu_Y\big]^2\right\rbrace  \\
		&\approx Var(\bar{d}) \\
		&=\left(1-\frac{n}{N}\right)\frac{\sigma_d^2}{n}
	\end{align*}
	其中：
	\begin{gather*}
		d_i=y_i-\big[\mu_Y+B_1(x_i-\mu_X)\big] \\
		\sigma_d^2=\frac{1}{N-1}\sum_{i=1}^N[y_i-\mu_Y-B_1(x_i-\mu_X)]^2=(1-R^2)\sigma_Y^2
	\end{gather*}
\end{theorem}
\begin{proof}
	下求$E(d)$：
	\begin{equation*}
		E(d)=\frac{1}{N}\left[\sum_{i=1}^Ny_i-N\mu_Y-B_1\sum_{i=1}^Nx_i+B_1N\mu_X\right]=0
	\end{equation*}
	因此：
	\begin{align*}
		\sigma_d^2&=\frac{1}{N-1}\sum_{i=1}^N\big[y_i-\mu_Y-B_1(x_i-\mu_X)\big]^2 \\
		&=\frac{1}{N-1}\left[\sum_{i=1}^N(y_i-\mu_Y)^2+\sum_{i=1}^NB_1^2(x_i-\mu_X)^2-\sum_{i=1}^N2B_i(y_i-\mu_Y)(x_i-\mu_X)\right] \\
		&=\sigma_Y^2+B_1^2\sigma_X^2-2B_1R\sigma_X\sigma_Y
	\end{align*}
	而：
	\begin{equation*}
		B_1=\frac{\sigma_YR}{\sigma_X}
	\end{equation*}
	所以：
	\begin{equation*}
		\sigma_d^2
		=\sigma_Y^2+B_1^2\sigma_X^2-2B_1R\sigma_X\sigma_Y 
		=\sigma_Y^2+\frac{\sigma_Y^2R^2}{\sigma_X^2}\sigma_X^2-2\frac{\sigma_YR}{\sigma_X}R\sigma_X\sigma_Y
		=\sigma_Y^2-R^2\sigma_Y^2
		=(1-R^2)\sigma_Y^2\qedhere
	\end{equation*}
\end{proof}
由此，在以下情况$MSE(\hat{\mu}_{Y_{reg}})$较小：
\begin{enumerate}
	\item $n$较大。
	\item $\frac{n}{N}$较大。
	\item $\sigma_Y$较小。
	\item $R$接近$\pm 1$。
\end{enumerate}


\subsection{比例估计量的均方误差}
\begin{theorem}
	比例估计量的均方误差为：
	\begin{align*}
		MSE(\hat{\mu}_{Yr})&\approx E\left[(\bar{y}-B\bar{x})^2\right] \\
		&=\left(1-\frac{n}{N}\right)\frac{\sigma_Y^2-2BR\sigma_X\sigma_Y+B^2\sigma_X^2}{n} \\
		&\approx Var(\hat{\mu}_{Yr})
	\end{align*}
\end{theorem}
证明过程可见David and Sukhatme, 1974。

